\message{ !name(<none>.tex)}
\message{ !name(<none>) !offset(10) }



\begin{align*}
    \psi(\nu) =& \frac {\nu \tau _{NMDA}}{1+ \nu \tau_{NMDA}}\bigg( 1+ \frac {1}{1+ \nu \tau_{NMDA}}\\
    &\times \sum_{n=1}^{\infty}\frac {(-\alpha \tau_{NMDA,rise})^nT_n}{(n+1)!} \bigg)
    %I don't understand what's wrong here
\end{align*}


\begin{align*}
    \tau_E =& \frac {C_m}{g_m S_E}\\
    S_E =& 1 + T_{E,ext}\nu_{ext} + T_{E,AMPA}\nu_E +(\rho _1 + \rho_2)\psi(\nu_E) + T_{EI}\nu_I\\
    \mu_E =& \frac{(T_{E,ext}\nu_{ext} + T_{E,AMPA}\nu_E + \rho_1\psi(\nu_E))(V_E - V_L)}{S_E}\\
\end{align*}
\begin{align*}
     +& \frac{\rho_2\psi(\nu_E)(\langle V \rangle - V_L) + T_{EI}\nu_I(V_I - V_L)}{S_E}\\
\end{align*}
\begin{align*}
    \langle\eta(t)\eta(t')\rangle =& \frac{1}{\tau_{AMPA}}\text{exp} \left( - \frac{|t-t'|}{\tau_{AMPA}} \right)\\
    T_{E,ext} =& \frac{g_{AMPA,ext}C_{ext}\tau_{AMPA}}{g_m}\\
    T_{E,AMPA} =& \frac{f_{AMPA,rec}C_{ext}\tau_{AMPA}}{g_m}\\
    \rho_1 =& \frac {g_{NMDA}C_{E}}{g_mJ}\\
    \rho_2 =& \beta \frac{g_{NMDA}C_E(\langle V \rangle - V_E) (J-1)}{g_mJ^2}\\
    T_{EI} =& \frac {g_{GABA}C_I \tau_{GABA}}{g_m}
\end{align*}

\begin{align*}
    \sigma_E^2 =& \frac{g_{AMPA,ext}^2 (\langle V
    \rangle-V_E)C_{ext}\nu_{ext}\tau_{AMPA}^2\tau_E}{g_m^2\tau_m^2}
\end{align*}

\end{document}

\message{ !name(<none>.tex) !offset(-37) }
